Updating sbmf2022 sas example

publications/sbmf2022/sas.thy
@@ -1,13 +1,23 @@
 theory sas
-imports DFP
+imports "../../CSP-Prover/CSP_F/CSP_F"
 begin
 
-typedef ActuatorId = "{1..4}::nat set"
+
+typedef ActuatorId = "{1..4}::nat set" morphisms to_nat to_ActuatorId
 by (auto)
 
-type_synonym displacement = int
-type_synonym angularVelocity = int
-type_synonym voltage = int
+setup_lifting type_definition_ActuatorId
+
+declare [[coercion to_ActuatorId]]
+
+code_thms to_ActuatorId
+
+
+type_synonym displacement = real
+type_synonym angularVelocity = real
+type_synonym voltage = real
+
+
 
 definition dMAX :: "displacement"
 where "dMAX = 40"
@@ -15,48 +25,105 @@ where "dMAX = 40"
 definition dMIN :: "displacement"
 where "dMIN = -40"
             
-fun gain :: "int $\times$ int $\Rightarrow$ int"
+fun gain :: "real \<times> real \<Rightarrow> real"
 where "gain(x,k) = x * k"
 
-fun saturate :: "displacement $\Rightarrow$ angularVelocity"
+fun saturate :: "real \<Rightarrow> real"
 where "saturate(x) = max dMIN (min x dMAX)"
 
-fun dOmega :: "displacement $\Rightarrow$ angularVelocity"
+fun dOmega :: "displacement \<Rightarrow> angularVelocity"
 where "dOmega(e) = saturate(gain(e,20))"
 
-fun disp :: "angularVelocity $\Rightarrow$ displacement"
-where "disp(v) = (* omitted *)"
+fun disp :: "angularVelocity \<Rightarrow> displacement"
+where "disp(v) = v / 20"
 
-fun modulate :: "voltage $\Rightarrow$ displacement"
-where "modulate(v) = (* omitted *)"
+fun modulate :: "voltage \<Rightarrow> displacement"
+where "modulate(v) = v / 10"
 
-fun senseVoltage :: "displacement $\Rightarrow$ voltage"
-where "senseVoltage(p) = (* omitted *)"
+fun senseVoltage :: "displacement \<Rightarrow> voltage"
+where "senseVoltage(p) = gain(p,10)"
+
+
+
+lemma modulate_senseVoltage [simp]: "(modulate (senseVoltage a)) = a"
+by (auto)
+
+lemma senseVoltage_modulate [simp]: "(senseVoltage (modulate a)) = a"
+by (auto)
+
+declare gain.simps [simp del]
+declare saturate.simps [simp del]
+declare dOmega.simps [simp del]
+declare disp.simps [simp del]
+declare modulate.simps [simp del]
+declare senseVoltage.simps [simp del]
+
 
 datatype Events = rawPosition ActuatorId displacement
                 | adjust ActuatorId displacement
                 | coreMoved ActuatorId displacement
                 | lvdtOutput ActuatorId voltage
+                | ehsvOutput ActuatorId displacement
+                | servoCmd ActuatorId displacement
+                | controlCmd ActuatorId displacement
+                | feedbackPos ActuatorId voltage
 
-datatype PN = Raw ActuatorId displacement displacement
-            | LVDT ActuatorId voltage
-            | SimpleActuator ActuatorId
+
+datatype PN = ACE ActuatorId
+            | EHSV ActuatorId
+            | Raw ActuatorId displacement
+            | LVDT ActuatorId
 
 
-primrec
-     PNfun :: "PN => (PN,Events) proc"
+primrec PNfun :: "PN \<Rightarrow> (PN,Events) proc"
 where
-    "PNfun(Raw i p adj) =
-           rawPosition(i)!p -> (let d = disp(dOmega(e))
-                                in $\$$(Raw i (p+d) (adj-d)))
-           [] adjust(i)?e -> $\$$(Raw i p e)"
-  | "PNfun(LVDT i v) =
-           lvdtOutput(i)!modulate(v) -> $\$$(LVDT i v)
-           [] coreMoved(i)?p -> $\$$(LVDT i senseVoltage(p))"
+    "PNfun(ACE i) =
+           controlCmd(i) ? p \<rightarrow> feedbackPos(i) ? feedback \<rightarrow> servoCmd(i) ! (saturate(p - feedback)) \<rightarrow> $ACE i"
+  | "PNfun(EHSV i) =
+           rawPosition(i) ? p \<rightarrow> servoCmd(i) ? e \<rightarrow> ehsvOutput(i) ! (p - disp (dOmega e)) \<rightarrow> $EHSV i"
+  | "PNfun(Raw i p) =
+           rawPosition(i) ! p \<rightarrow> $Raw i p
+           [+] adjust(i) ? adj \<rightarrow> $Raw i (saturate (p + adj))"
+  | "PNfun(LVDT i) =
+           coreMoved(i) ? p \<rightarrow> lvdtOutput(i) ! (modulate (senseVoltage p)) \<rightarrow> $LVDT i"
 
-  | "PNfun(SimpleActuator i) =
-           $\$$(Raw i 0 0)
-           [| \{| rawPosition |\} |]
-           ( $\$$(LVDT i 0) [[ coreMoved <- rawPosition ]] )"
+
+overloading Set_PNfun == 
+  "CSP_syntax.PNfun :: (PN,Events)pnfun"
+begin
+  definition "CSP_syntax.PNfun == PNfun::((PN,Events) pnfun)"
+end
+declare Set_PNfun_def [simp add]
+
+
+lemma guardedfun_PNfun [simp]: "guardedfun PNfun"
+  apply (simp add: guardedfun_def)
+  by (rule allI, induct_tac p, simp_all add: Let_def)
+
+
+
+definition PCU
+where "PCU i p0 ==
+            (
+              $EHSV i [[ ehsvOutput i <== adjust i ]]
+              |[ {| rawPosition i, adjust i |}\<^sub>c ]|
+              ( $Raw i p0 )
+            )
+            |[ {| rawPosition i |}\<^sub>c ]|
+            ( $LVDT i [[ coreMoved i <== rawPosition i ]] [[ lvdtOutput i <== feedbackPos i ]] )"
+
+
+definition ACE_PCU
+where "ACE_PCU i p0 ==
+           $ACE i
+           |[ {| servoCmd i, feedbackPos i |}\<^sub>c ]|
+           PCU i p0"
+
+
+definition SimpleActuator
+where "SimpleActuator i == ACE_PCU i 0"
+
+
+
 
 end
