publications/sbmf2022/PCU.thy
@@ -1,0 +1,244 @@
+theory pcu
+imports "df"
+begin
+
+
+typedef ActuatorId = "{1..4}::nat set" morphisms to_nat to_ActuatorId
+by (auto)
+
+setup_lifting type_definition_ActuatorId
+
+declare [[coercion to_ActuatorId]]
+
+code_thms to_ActuatorId
+
+
+type_synonym displacement = real
+type_synonym angularVelocity = real
+type_synonym voltage = real
+
+
+
+definition dMAX :: "displacement"
+where "dMAX = 40"
+
+definition dMIN :: "displacement"
+where "dMIN = -40"
+            
+fun gain :: "real \<times> real \<Rightarrow> real"
+where "gain(x,k) = x * k"
+
+fun saturate :: "real \<Rightarrow> real"
+where "saturate(x) = max dMIN (min x dMAX)"
+
+fun dOmega :: "displacement \<Rightarrow> angularVelocity"
+where "dOmega(e) = saturate(gain(e,20))"
+
+fun disp :: "angularVelocity \<Rightarrow> displacement"
+where "disp(v) = v / 20"
+
+fun modulate :: "voltage \<Rightarrow> displacement"
+where "modulate(v) = v / 10"
+
+fun senseVoltage :: "displacement \<Rightarrow> voltage"
+where "senseVoltage(p) = gain(p,10)"
+
+
+
+datatype Events = rawPosition ActuatorId displacement
+                | adjust ActuatorId displacement
+                | coreMoved ActuatorId displacement
+                | lvdtOutput ActuatorId voltage
+
+
+
+datatype PN = Raw ActuatorId displacement displacement
+            | LVDT ActuatorId voltage
+
+
+primrec PNfun :: "PN \<Rightarrow> (PN,Events) proc"
+where
+    "PNfun(Raw i p adj) =
+           rawPosition(i)!p \<rightarrow> (let d = disp(dOmega(adj))
+                                in $(Raw i (p+d) (adj-d)))
+           [+] adjust(i) ? e \<rightarrow> $(Raw i p e)"
+
+  | "PNfun(LVDT i v) =
+           lvdtOutput(i)!(modulate v) \<rightarrow> $(LVDT i v)
+           [+] coreMoved(i) ? p \<rightarrow> $(LVDT i (senseVoltage p))"
+
+
+overloading Set_PNfun == 
+  "CSP_syntax.PNfun :: (PN,Events)pnfun"
+begin
+  definition "CSP_syntax.PNfun == PNfun::((PN,Events) pnfun)"
+end
+declare Set_PNfun_def [simp add]
+
+
+lemma guardedfun_PNfun : "guardedfun PNfun"
+  apply (simp add: guardedfun_def)
+  apply (rule allI, induct_tac p)
+  apply (simp_all add: Let_def)
+done
+
+
+overloading Set_FPmode == 
+  "CSP_syntax.FPmode :: fpmode"
+begin
+  definition "CSP_syntax.FPmode == MIXmode"
+end
+declare Set_FPmode_def [simp add]
+
+
+
+definition ActuatorRawLVDT :: "ActuatorId \<Rightarrow> displacement \<Rightarrow> voltage \<Rightarrow> (PN,Events) proc"
+where "ActuatorRawLVDT i p v ==
+           $Raw i p 0
+           |[ {| rawPosition i |}\<^sub>c ]|
+           $LVDT i v [[ coreMoved i <== rawPosition i ]]"
+
+
+definition SimpleActuator :: "ActuatorId \<Rightarrow> (PN,Events) proc"
+where "SimpleActuator i == ActuatorRawLVDT i 0 0"
+
+
+
+
+
+
+fun DF_to_ActuatorRawLVDT :: "ActuatorId \<Rightarrow> DFtickName \<Rightarrow> (PN, Events) proc"
+where
+    "DF_to_ActuatorRawLVDT i (DFtick) =
+           !<rawPosition i> p .. !<adjust i> a .. !<lvdtOutput i> v ..
+           $Raw i p a
+           |[ {| rawPosition i |}\<^sub>c ]|
+           $LVDT i v [[ coreMoved i <== rawPosition i ]]"
+
+
+declare inj_def [simp add]
+
+declare gain.simps [simp del]
+declare saturate.simps [simp del]
+declare dOmega.simps [simp del]
+declare disp.simps [simp del]
+declare modulate.simps [simp del]
+declare senseVoltage.simps [simp del]
+
+
+
+lemma Lemma_DF_to_ActuatorRawLVDT :
+    "(DFtickfun p) << (DF_to_ActuatorRawLVDT i) <=F DF_to_ActuatorRawLVDT i p"
+  apply (induct_tac p, auto)
+  apply (cspF_auto)+
+  apply (rule cspF_Int_choice_left1)
+  apply (cspF_prefix_left)
+  apply (rule cspF_decompo_ref)
+  apply (force)
+  apply (force)
+
+  apply (cspF_auto)
+  apply (erule disjE)
+
+    apply (simp)
+    apply (cspF_auto)
+    apply (cspF_auto)
+    apply (simp add: image_def Let_def)
+    apply (cspF_auto_right)
+    apply (cspF_auto_right)
+    apply (cspF_auto_right)
+    apply (rule cspF_Rep_int_choice_left, simp)
+      apply (rule_tac x="(a + disp (dOmega aa))" in exI, simp)
+    apply (rule cspF_Rep_int_choice_left, simp)
+      apply (rule exI, simp)
+    apply (rule cspF_Rep_int_choice_left, simp)
+      apply (rule_tac x="senseVoltage (a)" in exI, simp)
+    apply (rule cspF_decompo, simp)
+    apply (rule cspF_decompo, simp add: Let_def)
+    apply (cspF_hsf_right)
+    apply (cspF_hsf_right, simp add: image_def)
+    apply (cspF_ren)
+
+    apply (simp add: image_def Let_def, auto)
+
+      apply (cspF_hsf_right)
+      apply (cspF_hsf_right)
+      apply (cspF_hsf_right)
+      apply (cspF_hsf_right)
+      apply (cspF_hsf_right)
+      apply (cspF_auto_right)
+      apply (rule cspF_Rep_int_choice_left, simp)
+        apply (rule_tac x="a" in exI, simp)
+      apply (rule cspF_Rep_int_choice_left, simp)
+        apply (rule exI, simp)
+      apply (rule cspF_Rep_int_choice_left, simp)
+        apply (rule_tac x="ab" in exI, simp)
+      apply (rule cspF_decompo, simp)
+      apply (rule cspF_decompo, simp add: Let_def)
+      apply (cspF_hsf_right)
+      apply (cspF_hsf)
+
+      apply (cspF_ren)
+      apply (cspF_hsf)
+      apply (cspF_hsf)
+      apply (cspF_hsf, simp add: Image_def)
+      apply (rule cspF_decompo, simp add: Renaming2_channel_def Renaming2_channel_fun_def fun_to_rel_def)
+      apply (auto)
+      apply (cspF_auto)
+      apply (simp add: Renaming2_channel_def Renaming2_channel_fun_def fun_to_rel_def)
+      apply (cspF_hsf)
+      apply (cspF_hsf)
+      apply (cspF_hsf)
+      apply (cspF_hsf)
+      apply (rule cspF_Rep_int_choice_left, simp)
+        apply (rule_tac x="x" in exI, simp)
+      apply (simp add: Renaming2_channel_def Renaming2_channel_fun_def fun_to_rel_def)
+
+      apply (cspF_hsf_right)
+      apply (cspF_hsf_right)
+      apply (cspF_hsf_right)
+      apply (cspF_hsf_right)
+      apply (cspF_hsf_right)
+      apply (cspF_auto_right)
+      apply (rule cspF_Rep_int_choice_left, simp)
+        apply (rule_tac x="a" in exI, simp)
+      apply (rule cspF_Rep_int_choice_left, simp)
+        apply (rule exI, simp)
+      apply (rule cspF_Rep_int_choice_left, simp)
+        apply (rule_tac x="ab" in exI, simp)
+      apply (rule cspF_decompo, simp)
+      apply (cspF_auto)
+      apply (cspF_auto)
+      apply (cspF_auto)
+      apply (rule cspF_decompo, simp add: image_def)
+      apply (cspF_auto)
+      apply (simp add: image_def)
+      apply (cspF_auto)+
+done
+
+
+lemma DF_ActuatorRawLVDT : " $DFtick <=F ((ActuatorRawLVDT i p v)::(PN,Events) proc)"
+  apply (rule_tac Pf="DFtickfun" and f="DF_to_ActuatorRawLVDT i" in cspF_fp_induct_ref_left)
+  apply (simp, simp, simp, simp)
+  apply (simp add: ActuatorRawLVDT_def)
+  apply (rule cspF_Rep_int_choice_left, simp)
+    apply (rule_tac  x="p" in exI, simp)
+  apply (rule cspF_Rep_int_choice_left, simp)
+    apply (rule_tac  x="0" in exI, simp)
+  apply (rule cspF_Rep_int_choice_left, simp)
+    apply (rule_tac  x="v" in exI, simp)
+by (rule Lemma_DF_to_ActuatorRawLVDT)
+
+
+theorem ActuatorRawLVDT_isDeadlockFree : "((ActuatorRawLVDT i p v)::(PN,Events) proc) isDeadlockFree"
+  apply (simp only: DeadlockFree_DFtick_ref)
+by (rule DF_ActuatorRawLVDT)
+
+
+theorem SimpleActuator_isDeadlockFree : "((SimpleActuator i)::(PN,Events) proc) isDeadlockFree"
+  apply (simp only: SimpleActuator_def)
+by (rule ActuatorRawLVDT_isDeadlockFree)
+
+
+
+end
