publications/sbmf2022/sas_df.thy
@@ -1,0 +1,533 @@
+theory sas_df
+imports "sas_analysis"
+        "CSP_F.CSP_F_law_step_aux"
+        "DFP_DFfive"
+begin
+
+
+overloading Set_FPmode == 
+  "CSP_syntax.FPmode :: fpmode"
+begin
+  definition "CSP_syntax.FPmode == CMSmode"
+end
+declare Set_FPmode_def [simp add]
+
+
+
+declare inj_def [simp add]
+declare Let_def [simp add]
+
+declare Rec_prefix_def [simp add]
+declare Send_prefix_def [simp add]
+
+fun DFfive_to_ACE_PCUadj :: "ActuatorId \<Rightarrow> DFfivePN \<Rightarrow> (PN, Events) proc"
+where
+    "DFfive_to_ACE_PCUadj i (DFfive) =
+           (!<adjust i> adj .. !<rawPosition i> p0 ..
+             $ACE i
+             |[ {| servoCmd i, feedbackPos i |}\<^sub>c ]|
+             PCUadj i p0 adj)"
+
+
+lemma Lemma_DFfive_to_ACE_PCUadj :
+    "(DFfivefun p) << (DFfive_to_ACE_PCUadj i) <=F DFfive_to_ACE_PCUadj i p"
+  apply (induct_tac p)
+  apply (auto)
+
+  (* Expand RIGHT *)
+  apply (rule cspF_rw_right, rule unwind_ACE_PCUadj)
+  apply (rule cspF_rw_right, rule cspF_Parallel_step_choice)
+    apply (rule cspF_reflex, rule cspF_reflex, simp)
+    apply (cspF_simp_right)
+
+  (* STEP - controlCmd OR adjust is the 1\<ordmasculine> event *)
+  apply (rule cspF_Ext_choice_right)
+  
+    (* REFINED - controlCmd is the 1\<ordmasculine> event *)
+    apply (cspF_step_left)
+    apply (rule cspF_decompo_ref, simp, simp)
+    apply (erule rangeE, simp)
+
+      (* Expand RIGHT *)
+      apply (rule cspF_rw_right, rule cspF_Parallel_step_choice)
+        apply (rule cspF_reflex, rule cspF_reflex, simp)
+        apply (cspF_simp_right)
+        apply (cspF_simp_right)
+  
+      (* REFINED - adjust is the 2\<ordmasculine> event *)
+      apply (cspF_step_left)
+      apply (rule cspF_decompo_ref, simp, simp)
+      apply (simp)
+  
+      (* Expand RIGHT *)
+      apply (rule cspF_rw_right, rule cspF_Parallel_step_choice)
+        apply (rule cspF_reflex)
+        apply (rule cspF_rw_left, rule cspF_Parallel_step_choice)
+          apply (rule cspF_rw_left, rule cspF_Parallel_step_choice)
+            apply (rule unwind_EHSV)
+            apply (rule cspF_rw_left, rule unwind_Raw)
+            apply (rule cspF_Ext_choice_step_Ext_pre_choice_disjnt, simp add: disjnt_def)
+            apply (simp)
+            apply (cspF_simp_left)
+            apply (cspF_simp_left)
+          apply (rule unwind_LVDT)
+          apply (simp)
+          apply (cspF_simp_left)
+          apply (cspF_simp_left)
+        apply (cspF_simp_right)
+        apply (cspF_simp_right)
+    
+      (* REFINED - rawPosition is the 3\<ordmasculine> event *)
+      apply (cspF_step_left)
+      apply (rule cspF_decompo_ref, simp, simp)
+      apply (simp)
+  
+      (* Expand RIGHT *)
+      apply (rule cspF_rw_right, rule cspF_Parallel_step_choice)
+        apply (rule cspF_reflex, simp)
+        apply (rule cspF_rw_left, rule cspF_Parallel_step_choice)
+          apply (rule cspF_rw_left, rule cspF_Parallel_step_choice)
+          apply (rule cspF_reflex, cspF_simp_left)
+          apply (rule cspF_Ext_choice_step_Ext_pre_choice_disjnt, simp add: disjnt_def)
+          apply (simp)
+          apply (cspF_simp_left)
+          apply (cspF_simp_left)
+        apply (rule cspF_Ext_choice_step_Ext_pre_choice_disjnt, simp add: disjnt_def)
+        apply (simp)
+        apply (cspF_simp_right)
+        apply (cspF_simp_right)
+  
+      (* REFINED - feedbackPos is the 5\<ordmasculine> event *)
+      apply (cspF_step_left)
+      apply (rule cspF_decompo_ref, simp, simp)
+      apply (simp)
+  
+      (* Expand RIGHT *)
+      apply (rule cspF_rw_right, rule cspF_Parallel_step_choice)
+        apply (rule cspF_reflex)
+        apply (cspF_simp_left)
+        apply (rule cspF_rw_left, rule cspF_Parallel_step_choice)
+          apply (rule cspF_reflex, rule unwind_LVDT, simp)
+          apply (cspF_simp_left)
+          apply (cspF_simp_left)
+        apply (cspF_simp_right)
+        apply (cspF_simp_right)
+  
+      (* REFINED - servoCmd is the 6\<ordmasculine> event *)
+      apply (cspF_step_left)
+      apply (rule cspF_decompo_ref, simp, simp)
+      apply (simp)
+  
+      apply (rule cspF_Rep_int_choice_left, simp)
+      apply (rule_tac x="(saturate (aa + a) - disp (dOmega (saturate (x - saturate (aa + a)))))" in exI, simp)
+      apply (rule cspF_Rep_int_choice_left, simp)
+      apply (rule_tac x="(saturate (aa + a))" in exI, simp)
+  
+      apply (rule cspF_decompo, simp, simp)
+  
+      (* Expand RIGHT *)
+      apply (rule cspF_rw_right, rule cspF_Parallel_step_choice)
+        apply (rule cspF_rw_left, rule cspF_Parallel_step_choice)
+          apply (rule cspF_reflex, rule cspF_reflex, simp)
+          apply (cspF_simp_left)
+          apply (cspF_simp_left)
+        apply (cspF_simp_right)
+        apply (cspF_simp_right)
+  
+      apply (simp add: PCUadj_def)
+      apply (rule cspF_decompo, simp, simp)
+      apply (rule cspF_decompo, simp)
+      apply (rule cspF_decompo, simp, simp)
+      apply (rule cspF_rw_right, rule cspF_IF, simp)
+      apply (rule cspF_eq_ref, rule unwind_LVDT)
+
+    (* REFINED - adjust is the 1\<ordmasculine> event *)
+    apply (cspF_step_left)
+    apply (rule cspF_decompo_ref, simp, simp)
+    apply (simp)
+
+      (* Expand RIGHT *)
+      apply (rule cspF_rw_right, rule cspF_Parallel_step_choice)
+        apply (rule cspF_reflex)
+        apply (rule cspF_rw_left, rule cspF_Parallel_step_choice)
+          apply (rule cspF_rw_left, rule cspF_Parallel_step_choice)
+          apply (rule unwind_EHSV)
+          apply (rule cspF_rw_left, rule unwind_Raw)
+          apply (rule cspF_Ext_choice_step_Ext_pre_choice_disjnt, simp add: disjnt_def)
+          apply (simp)
+          apply (cspF_simp_left)
+          apply (cspF_simp_left)
+        apply (rule unwind_LVDT)
+        apply (simp)
+        apply (cspF_simp_left)
+        apply (cspF_simp_left)
+      apply (cspF_simp_right)
+  
+      (* STEP - controlCmd OR rawPosition is the 2\<ordmasculine> event *)
+      apply (rule cspF_Ext_choice_right)
+  
+      (* REFINED - controlCmd is the 2\<ordmasculine> event *)
+      apply (cspF_step_left)
+      apply (rule cspF_decompo_ref, simp, simp)
+      apply (erule rangeE, simp)
+
+        (* Expand RIGHT *)
+        apply (rule cspF_rw_right, rule cspF_Parallel_step_choice)
+          apply (rule cspF_reflex, rule cspF_reflex, simp)
+        apply (cspF_simp_right)
+        apply (cspF_simp_right)
+
+        (* REFINED - rawPosition is the 3\<ordmasculine> event *)
+        apply (cspF_step_left)
+        apply (rule cspF_decompo_ref, simp, simp)
+        apply (simp)
+
+        (* Expand RIGHT *)
+        apply (rule cspF_rw_right, rule cspF_Parallel_step_choice)
+          apply (rule cspF_reflex)
+          apply (rule cspF_rw_left, rule cspF_Parallel_step_choice)
+            apply (rule cspF_rw_left, rule cspF_Parallel_step_choice)
+            apply (rule cspF_reflex, cspF_simp_left)
+            apply (rule cspF_Ext_choice_step_Ext_pre_choice_disjnt, simp add: disjnt_def)
+            apply (simp)
+              apply (cspF_simp_left)
+              apply (cspF_simp_left)
+          apply (rule cspF_Ext_choice_step_Ext_pre_choice_disjnt, simp add: disjnt_def)
+          apply (simp)
+        apply (cspF_simp_right)
+        apply (cspF_simp_right)
+    
+        (* REFINED - feedbackPos is the 4\<ordmasculine> event *)
+        apply (cspF_step_left)
+        apply (rule cspF_decompo_ref, simp, simp)
+        apply (simp)
+    
+        (* Expand RIGHT *)
+        apply (rule cspF_rw_right, rule cspF_Parallel_step_choice)
+          apply (rule cspF_reflex, cspF_simp_left)
+          apply (rule cspF_rw_left, rule cspF_Parallel_step_choice)
+          apply (rule cspF_reflex, rule unwind_LVDT, simp)
+          apply (cspF_simp_left)
+          apply (cspF_simp_left)
+        apply (cspF_simp_right)
+        apply (cspF_simp_right)
+    
+        (* REFINED - servoCmd is the 5\<ordmasculine> event *)
+        apply (cspF_step_left)
+        apply (rule cspF_decompo_ref, simp, simp)
+        apply (simp)
+
+        apply (rule cspF_Rep_int_choice_left, simp)
+        apply (rule_tac x="saturate (aa + a) - disp (dOmega (saturate (x - saturate (aa + a))))" in exI, simp)
+        apply (rule cspF_Rep_int_choice_left, simp)
+        apply (rule_tac x="(saturate (aa + a))" in exI, simp)
+    
+        apply (rule cspF_decompo, simp, simp)
+    
+        (* Expand RIGHT *)
+        apply (rule cspF_rw_right, rule cspF_Parallel_step_choice)
+          apply (rule cspF_rw_left, rule cspF_Parallel_step_choice)
+            apply (rule cspF_reflex, rule cspF_reflex, simp)
+            apply (cspF_simp_left)
+            apply (cspF_simp_left)
+          apply (cspF_simp_right)
+          apply (cspF_simp_right)
+  
+        (* REFINED *)
+        apply (simp add: PCUadj_def)
+        apply (rule cspF_decompo, simp, simp)
+        apply (rule cspF_decompo, simp)
+        apply (rule cspF_decompo, simp, simp)
+        apply (rule cspF_rw_right, rule cspF_IF, simp)
+        apply (rule cspF_eq_ref, rule unwind_LVDT)
+
+      (* REFINED - rawPosition is the 2\<ordmasculine> event *)
+      apply (cspF_step_left)
+      apply (rule cspF_decompo_ref, simp, simp)
+      apply (simp)
+
+        (* Expand RIGHT *)
+        apply (rule cspF_rw_right, rule cspF_Parallel_step_choice)
+          apply (rule cspF_reflex)
+          apply (rule cspF_rw_left, rule cspF_Parallel_step_choice)
+            apply (rule cspF_rw_left, rule cspF_Parallel_step_choice)
+            apply (rule cspF_reflex)
+            apply (cspF_simp_left)
+            apply (rule cspF_Ext_choice_step_Ext_pre_choice_disjnt, simp add: disjnt_def)
+            apply (simp)
+            apply (cspF_simp_left)
+            apply (cspF_simp_left)
+          apply (rule cspF_Ext_choice_step_Ext_pre_choice_disjnt, simp add: disjnt_def)
+          apply (simp)
+        apply (cspF_simp_right)
+        apply (cspF_simp_right)
+    
+        (* REFINED - controlCmd is the 3\<ordmasculine> event *)
+        apply (cspF_step_left)
+        apply (rule cspF_decompo_ref, simp, simp)
+        apply (erule rangeE, simp)
+  
+        (* Expand RIGHT *)
+        apply (rule cspF_rw_right, rule cspF_Parallel_step_choice)
+          apply (rule cspF_reflex, rule cspF_reflex, simp)
+        apply (cspF_simp_right)
+        apply (cspF_simp_right)
+    
+        (* REFINED - feedbackPos is the 4\<ordmasculine> event *)
+        apply (cspF_step_left)
+        apply (rule cspF_decompo_ref, simp, simp)
+        apply (simp)
+    
+        (* Expand RIGHT *)
+        apply (rule cspF_rw_right, rule cspF_Parallel_step_choice)
+        apply (rule cspF_reflex)
+        apply (rule cspF_rw_left, rule cspF_IF)
+        apply (rule cspF_rw_left, rule cspF_Parallel_step_choice)
+        apply (rule cspF_reflex)
+        apply (rule unwind_LVDT)
+        apply (simp)
+        apply (cspF_simp_left)
+        apply (cspF_simp_left)
+        apply (cspF_simp_right)
+        apply (cspF_simp_right)
+    
+        (* REFINED - servoCmd is the 5\<ordmasculine> event *)
+        apply (cspF_step_left)
+        apply (rule cspF_decompo_ref, simp, simp)
+        apply (simp)
+    
+        apply (rule cspF_Rep_int_choice_left, simp)
+        apply (rule_tac x="(saturate (aa + a) - disp (dOmega (saturate (x - saturate (aa + a)))))" in exI, simp)
+        apply (rule cspF_Rep_int_choice_left, simp)
+        apply (rule_tac x="(saturate (aa + a))" in exI, simp)
+    
+        apply (rule cspF_decompo, simp, simp)
+    
+        (* Expand RIGHT *)
+        apply (rule cspF_rw_right, rule cspF_Parallel_step_choice)
+        apply (rule cspF_rw_left, rule cspF_Parallel_step_choice)
+        apply (rule cspF_reflex)
+        apply (rule cspF_reflex)
+        apply (simp)
+        apply (rule cspF_rw_left, rule cspF_Ext_choice_unit_r_hsf)
+        apply (rule cspF_rw_left, rule cspF_Ext_choice_unit_r_hsf)
+        apply (rule cspF_reflex)
+        apply (rule cspF_reflex)
+        apply (simp)
+        apply (cspF_simp_right)
+        apply (cspF_simp_right)
+  
+        (* REFINED *)
+        apply (simp add: PCUadj_def)
+        apply (rule cspF_decompo, simp, simp)
+        apply (rule cspF_decompo, simp)
+        apply (rule cspF_decompo, simp, simp)
+        apply (rule cspF_rw_right, rule cspF_IF, simp)
+        apply (rule cspF_eq_ref, rule unwind_LVDT)
+done
+
+
+
+lemma DFtick_ACE_PCUadj : "$DFtick <=F ((ACE_PCUadj i p adj)::(PN,Events) proc)"
+  apply (rule cspF_trans, rule DFtick_DFfive)
+  apply (rule_tac Pf="DFfivefun" and f="DFfive_to_ACE_PCUadj i" in cspF_fp_induct_ref_left)
+  apply (simp, simp, simp, simp)
+  apply (rule cspF_Rep_int_choice_left, simp)
+    apply (rule_tac  x="adj" in exI, simp)
+  apply (rule cspF_Rep_int_choice_left, simp)
+    apply (rule_tac  x="p" in exI, simp)
+  apply (simp add: ACE_PCUadj_def)
+  by (rule Lemma_DFfive_to_ACE_PCUadj)
+
+
+
+lemma DF_ACE_PCU : "$DFtick <=F ((ACE_PCU i p)::(PN,Events) proc)"
+  (* Expand RIGHT *)
+  apply (rule cspF_rw_right, rule unwind_ACE_PCU)
+    apply (rule cspF_rw_right, rule cspF_Parallel_step_choice)
+      apply (rule cspF_reflex)
+      (* PCU = ( EHSV |[ ... ]| Raw ) |[ ... ]| LVDT *)
+      apply (rule cspF_rw_left, rule cspF_Parallel_step_choice)
+       apply (rule cspF_rw_left, rule cspF_Parallel_step_choice)
+        apply (rule cspF_reflex)
+        apply (rule cspF_Ext_choice_step_Ext_pre_choice_disjnt, simp add: disjnt_def)
+        apply (simp)
+       apply (cspF_simp_left)
+        apply (cspF_simp_left)
+        apply (cspF_simp_left)
+        apply (cspF_simp_right)
+    apply (rule cspF_rw_right, rule cspF_Ext_choice_step_Ext_pre_choice_disjnt, simp add: disjnt_def)
+
+    (* 1\<ordmasculine> STEP IS REFINED - rawPosition OR controlCmd is the first event*)
+    apply (cspF_unwind_left, cspF_step_left, rule cspF_Int_choice_left1)
+    apply (rule cspF_decompo_ref, simp, simp)
+    apply (clarsimp, erule disjE)
+
+    (* rawPosition is the first event *)
+    apply (simp)
+    apply (cspF_simp_right)
+    apply (cspF_simp_right)
+
+      (* Expand RIGHT *)
+      apply (rule cspF_rw_right, rule cspF_Parallel_step_choice)
+        apply (rule cspF_reflex)
+        apply (rule cspF_rw_left, rule cspF_Parallel_step_choice)
+        apply (rule cspF_rw_left, rule cspF_Parallel_step_choice)
+          apply (rule cspF_reflex)
+          apply (rule cspF_Ext_choice_step_Ext_pre_choice_disjnt, simp add: disjnt_def)
+          apply (simp)
+        apply (cspF_simp_left)
+        apply (cspF_simp_left)
+      apply (rule cspF_Ext_choice_step_Ext_pre_choice_disjnt, simp add: disjnt_def)
+      apply (simp)
+      apply (cspF_simp_right)
+      apply (cspF_simp_right)
+
+      (* 2\<ordmasculine> STEP IS REFINED - controlCmd is the second event *)
+      apply (cspF_unwind_left, cspF_step_left, rule cspF_Int_choice_left1)
+      apply (rule cspF_decompo_ref, simp, simp)
+      apply (erule rangeE, simp)
+  
+      (* Expand RIGHT *)
+      apply (rule cspF_rw_right, rule cspF_Parallel_step_choice)
+        apply (rule cspF_reflex, rule cspF_reflex, simp)
+      apply (cspF_simp_right)
+      apply (cspF_simp_right)
+  
+      (* 3\<ordmasculine> STEP IS REFINED - feedbackPos is the third event *)
+      apply (cspF_unwind_left, cspF_step_left, rule cspF_Int_choice_left1)
+      apply (rule cspF_decompo_ref, simp, simp)
+      apply (simp)
+
+      (* Expand RIGHT *)
+      apply (rule cspF_rw_right, rule cspF_Parallel_step_choice)
+        apply (rule cspF_reflex, cspF_simp_left)
+        apply (rule cspF_rw_left, rule cspF_Parallel_step_choice)
+        apply (rule cspF_reflex, rule unwind_LVDT, simp)
+        apply (cspF_simp_left)
+        apply (cspF_simp_left)
+      apply (cspF_simp_right)
+      apply (cspF_simp_right)
+  
+      (* 4\<ordmasculine> STEP IS REFINED - servoCmd is the fourth event *)
+      apply (cspF_unwind_left, cspF_step_left, rule cspF_Int_choice_left1)
+      apply (rule cspF_decompo_ref, simp, simp)
+      apply (simp)
+
+      (* REFINED BY TRANS DFtick_ACE_PCUadj *)
+      apply (rule cspF_trans)
+      apply (rule_tac i="i" and p="p" and adj="(p - disp (dOmega (saturate (x - p))))" in DFtick_ACE_PCUadj)
+      apply (simp add: ACE_PCUadj_def)
+      apply (rule cspF_decompo, simp, simp)
+      apply (simp add: PCUadj_def)
+
+      (* Expand RIGHT *)
+      apply (rule cspF_rw_right, rule cspF_Parallel_step_choice)
+      apply (rule cspF_rw_left, rule cspF_Parallel_step_choice)
+       apply (rule cspF_reflex, rule cspF_reflex, simp)
+        apply (cspF_simp_left)
+        apply (cspF_simp_left)
+      apply (cspF_simp_right)
+      apply (cspF_simp_right)
+
+      (* REFINED BY DECOMPO *)
+      apply (rule cspF_decompo, simp, simp)
+      apply (rule cspF_decompo, simp)
+      apply (rule cspF_decompo, simp, simp)
+      apply (cspF_simp_right)
+      apply (rule cspF_eq_ref, rule unwind_LVDT)
+
+
+    (* controlCmd is the first event *)
+    apply (cspF_simp_right)
+    apply (erule rangeE, simp)
+
+      (* Expand RIGHT *)
+      apply (rule cspF_rw_right, rule cspF_Parallel_step_choice)
+      apply (rule cspF_reflex, rule cspF_reflex, simp)
+      apply (cspF_simp_right)
+      apply (cspF_simp_right)
+
+      (* 2\<ordmasculine> STEP IS REFINED - rawPosition is the second event *)
+      apply (cspF_unwind_left, cspF_step_left, rule cspF_Int_choice_left1)
+      apply (rule cspF_decompo_ref, simp, simp)
+      apply (simp)
+  
+      (* Expand RIGHT *)
+      apply (rule cspF_rw_right, rule cspF_Parallel_step_choice)
+        apply (rule cspF_reflex)
+        apply (rule cspF_rw_left, rule cspF_Parallel_step_choice)
+        apply (rule cspF_rw_left, rule cspF_Parallel_step_choice)
+          apply (rule cspF_reflex)
+          apply (rule cspF_rw_left, rule cspF_IF)
+            apply (rule cspF_Ext_choice_step_Ext_pre_choice_disjnt, simp add: disjnt_def)
+          apply (simp)
+        apply (cspF_simp_left)
+        apply (cspF_simp_left)
+        apply (rule cspF_Ext_choice_step_Ext_pre_choice_disjnt, simp add: disjnt_def)
+        apply (simp)
+      apply (cspF_simp_right)
+      apply (cspF_simp_right)
+
+      (* 3\<ordmasculine> STEP IS REFINED - feedbackPos is the third event *)
+      apply (cspF_unwind_left, cspF_step_left, rule cspF_Int_choice_left1)
+      apply (rule cspF_decompo_ref, simp, simp)
+      apply (simp)
+
+      (* Expand RIGHT *)
+      apply (rule cspF_rw_right, rule cspF_Parallel_step_choice)
+        apply (rule cspF_reflex, cspF_simp_left)
+      apply (rule cspF_rw_left, rule cspF_Parallel_step_choice)
+        apply (rule cspF_reflex, rule unwind_LVDT, simp)
+      apply (cspF_simp_left)
+      apply (cspF_simp_left)
+      apply (cspF_simp_right)
+      apply (cspF_simp_right)
+
+      (* 4\<ordmasculine> STEP IS REFINED - servoCmd is the fourth event *)
+      apply (cspF_unwind_left, cspF_step_left, rule cspF_Int_choice_left1)
+      apply (rule cspF_decompo_ref, simp, simp)
+      apply (simp)
+
+      (* REFINED BY TRANS DFtick_ACE_PCUadj *)
+      apply (rule cspF_trans)
+      apply (rule_tac i="i" and p="p" and adj="(p - disp (dOmega (saturate (x - p))))" in DFtick_ACE_PCUadj)
+      apply (simp add: ACE_PCUadj_def)
+      apply (rule cspF_decompo, simp, simp)
+      apply (simp add: PCUadj_def)
+
+      (* Expand RIGHT *)
+      apply (rule cspF_rw_right, rule cspF_Parallel_step_choice)
+        apply (rule cspF_rw_left, rule cspF_Parallel_step_choice)
+         apply (rule cspF_reflex, rule cspF_reflex, simp)
+        apply (cspF_simp_left)
+        apply (cspF_simp_left)
+      apply (cspF_simp_right)
+      apply (cspF_simp_right)
+
+      (* REFINED BY DECOMPO *)
+      apply (rule cspF_decompo, simp, simp)
+      apply (rule cspF_decompo, simp)
+      apply (rule cspF_decompo, simp, simp)
+      apply (cspF_simp_right)
+      apply (rule cspF_eq_ref, rule unwind_LVDT)
+  done
+
+lemma DF_ACE_PCU_isDeadlockFree : "((ACE_PCU i p)::(PN,Events) proc) isDeadlockFree"
+  apply (simp only: DeadlockFree_DFtick_ref)
+  by (rule DF_ACE_PCU)
+
+
+theorem SimpleActuator_isDeadlockFree : "((SimpleActuator i)::(PN,Events) proc) isDeadlockFree"
+  apply (simp only: SimpleActuator_def)
+  by (rule DF_ACE_PCU_isDeadlockFree)
+
+
+
+declare inj_def [simp del]
+declare Let_def [simp del]
+
+declare Rec_prefix_def [simp del]
+declare Send_prefix_def [simp del]
+
+end
