publications/sbmf2022/SASinSimulink.md
@@ -2,7 +2,7 @@
 
 ---
 
-The Simulink model is provided [HERE](sas.mdl).
+The Simulink model is provided [HERE](SASdiscrete.mdl).
 
 The SAS *Simulink* model in order to allow simulation execution is presented below:
 
